src/Common/Equality.v
@@ -1,0 +1,68 @@
+Require Import Coq.Lists.List.
+
+Set Implicit Arguments.
+
+Definition pr1_path {A} {P : A -> Type} {u v : sigT P} (p : u = v)
+: projT1 u = projT1 v
+  := f_equal (@projT1 _ _) p.
+
+Definition pr2_path {A} {P : A -> Type} {u v : sigT P} (p : u = v)
+: eq_rect _ _ (projT2 u) _ (pr1_path p) = projT2 v.
+Proof.
+  destruct p; reflexivity.
+Defined.
+
+Lemma in_map_iff_injective {A B} (f : A -> B) (l : list A) (y : A)
+      (f_injective : forall x, f x = f y -> x = y)
+: In (f y) (map f l) <-> In y l.
+Proof.
+  split; intro H.
+  { apply in_map_iff in H.
+    destruct H as [x [H H']].
+    apply f_injective in H.
+    subst; assumption. }
+  { apply in_map_iff.
+    exists y; split; trivial. }
+Qed.
+
+Section option.
+  Context {A : Type}.
+
+  Definition option_code (x y : option A) : Prop
+    := match x, y with
+         | Some x', Some y' => x' = y'
+         | None, None => True
+         | _, _ => False
+       end.
+
+  Definition option_code_idpath {x} : option_code x x
+    := match x return option_code x x with
+         | Some _ => eq_refl
+         | None => I
+       end.
+
+  Definition option_encode {x y} (p : x = y) : option_code x y
+    := eq_rect _ _ option_code_idpath _ p.
+
+  Definition option_decode {x y} : option_code x y -> x = y
+    := match x, y return option_code x y -> x = y with
+         | Some x', Some y' => @f_equal _ _ (@Some _) _ _
+         | None, None => fun _ => eq_refl
+         | _, _ => fun H => match H : False with end
+       end.
+
+  Definition option_deenecode {x y} (p : x = y)
+  : option_decode (option_encode p) = p.
+  Proof.
+    destruct p, x; reflexivity.
+  Defined.
+
+  Definition option_endecode {x y} (p : option_code x y)
+  : option_encode (option_decode p) = p.
+  Proof.
+    destruct x, y, p; reflexivity.
+  Defined.
+
+  Definition Some_injective {x y : A} : Some x = Some y -> x = y
+    := option_encode.
+End option.
